src/basic/FStarC.Errors.Codes.fst
@@ -379,4 +379,5 @@ let default_settings : list error_setting =
     Error_CustardEntryNotFound                        , CAlwaysError, 362;
     Error_CustardCannotMonomorphize                   , CAlwaysError, 363;
     Error_CustardFuelExhausted                        , CAlwaysError, 364;
+    Error_CustardUnextractableEffect                  , CAlwaysError, 365;
     ]
